

Informal Derivation of Euler's Identity

David Rosenman

August 2, 2018

"Who would have thought that π which enters as the ratio of circumference to diameter, e , as the natural base for logarithms, i , as the fundamental imaginary unit and 0 and 1 (which we know all about from infancy) would all be tied together in any way, not to mention such a simple and compact way? I hope I never stumble into anything like this formula, for nothing I do after that in life would have any significance."

— Ramamurti Shankar

The Nobel Prize winning physicist Richard Feynman called equation (1), known as Euler's identity, "one of the most remarkable, almost astounding, formulas in all of mathematics."

$$e^{i\pi} + 1 = 0 \tag{1}$$

Euler's identity can be derived easily from the Taylor series...

$$f(x) = \sum_{n=0}^{\infty} \frac{f^{(n)}(0)}{n!} x^n \tag{2}$$

...as well as defining e^{ax} as

$$e^{ax} = \sum_{n=0}^{\infty} \frac{(ax)^n}{n!} \tag{3}$$

In equation (2), $f^{(n)}$ represents the n -th derivative of the function f , with the zeroth derivative of f being equal to f .

The Taylor series of $\cos(x)$ can be easily derived from equation (2).

$$\begin{aligned} f^0(x) &= f(x) = \cos x \\ f^0(0) &= f(0) = \cos 0 = 1 \\ f^1(x) &= \frac{df(x)}{dx} = \frac{d}{dx} \cos x = -\sin x \\ f^1(0) &= -\sin 0 = 0 \\ f^2(x) &= \frac{d^2f(x)}{dx^2} = -\frac{d}{dx} \sin x = -\cos x \\ f^2(0) &= -\cos 0 = -1 \\ f^3(x) &= -\frac{d}{dx} \cos x = \sin x \\ f^3(0) &= \sin 0 = 0 \\ f^4(x) &= \frac{d}{dx} \sin x = \cos x \\ f^4(0) &= \cos 0 = 1 \end{aligned}$$

From the equations above, as well at equation (2), it follows that:

$$\cos x = 1 - \frac{x^2}{2!} + \frac{x^4}{4!} - \dots = \sum_{n=0}^{\infty} \frac{(-1)^n}{(2n)!} x^{2n} \quad (4)$$

The Taylor series of $\sin x$ can also be derived equation from equation (2).

$$\begin{aligned} f^0(x) &= f(x) = \sin x \\ f^0(0) &= \sin 0 = 0 \\ f^1(x) &= \frac{d}{dx} \sin x = \cos x \\ f^1(0) &= \cos 0 = 1 \\ f^2(x) &= \frac{d}{dx} \cos x = -\sin x \\ f^2(0) &= -\sin 0 = 0 \\ f^3(x) &= -\frac{d}{dx} \sin x = -\cos x \\ f^3(0) &= -\cos 0 = -1 \\ f^4(x) &= -\frac{d}{dx} \cos x = \sin x \\ f^4(0) &= \sin 0 = 0 \\ f^5(x) &= \frac{d}{dx} \sin x = \cos x \\ f^5(0) &= \cos 0 = 1 \end{aligned}$$

From the equations above and equation (2), it follows that:

$$\sin x = x - \frac{x^3}{3!} + \frac{x^5}{5!} - \dots = \sum_{n=0}^{\infty} \frac{(-1)^n}{(2n+1)!} x^{2n+1} \quad (5)$$

From equations (3), (4), and (5), if θ is a real number:

$$\begin{aligned} e^{i\theta} &= \sum_{n=0}^{\infty} \frac{(i\theta)^n}{n!} = 1 + i\theta + \underbrace{i^2 \frac{\theta^2}{2!}}_{-1} + \underbrace{i^3 \frac{\theta^3}{3!}}_{-i} + \underbrace{i^4 \frac{\theta^4}{4!}}_1 + \underbrace{i^5 \frac{\theta^5}{5!}}_i - \dots \\ e^{i\theta} &= 1 + i\theta - \frac{\theta^2}{2!} - \frac{i\theta^3}{3!} + \frac{\theta^4}{4!} + \frac{i\theta^5}{5!} - \dots \\ e^{i\theta} &= \underbrace{\left(1 - \frac{\theta^2}{2!} + \frac{\theta^4}{4!} - \dots\right)}_{\cos \theta} + i \underbrace{\left(\theta - \frac{\theta^3}{3!} + \frac{\theta^5}{5!} - \dots\right)}_{\sin \theta} = \cos \theta + i \sin \theta \end{aligned} \quad (6)$$

Finally, let $\theta = \pi$. Equation (6) becomes:

$$e^{i\pi} = \cos \pi + i \sin \pi = -1$$

And finally:

$$\boxed{e^{i\pi} + 1 = 0}$$

References

1. Ramamurti Shankar, *Principles of Quantum Mechanics*. Springer, 1994.
2. James Stewart, *Calculus: Early Transcendentals*. Cengage Learning, 2012.